[WIP] shifting adds

src/Experiments/SimplyTypedArithmetic.v
@@ -8547,16 +8547,13 @@ Module PreFancy.
       Local Notation Z := (type.type_primitive type.Z).
 
       Inductive ident : type -> type -> Type :=
-      | add : ident (Z * Z) (Z * Z)
-      | addc : ident (Z * Z * Z) (Z * Z)
+      | add (imm : BinInt.Z) : ident (Z * Z) (Z * Z)
+      | addc (imm : BinInt.Z) : ident (Z * Z * Z) (Z * Z)
+      | sub (imm : BinInt.Z) : ident (Z * Z) (Z * Z)
       | mulll : ident (Z * Z) Z
       | mullh : ident (Z * Z) Z
       | mulhl : ident (Z * Z) Z
       | mulhh : ident (Z * Z) Z
-      | sub : ident (Z * Z) (Z * Z)
-      (* | land : BinInt.Z -> ident Z Z *)
-      | shiftr : BinInt.Z -> ident Z Z
-      | shiftl : BinInt.Z -> ident Z Z
       | rshi : BinInt.Z -> ident (Z * Z) Z
       | selc : ident (Z * Z * Z) Z
       | selm : ident (Z * Z * Z) Z
@@ -8649,27 +8646,70 @@ Module PreFancy.
         | _ => None
         end.
 
+      Definition invert_shift {t} (s : @scalar var t)
+        : option (@scalar var Z * BinInt.Z) :=
+          match s return option (@scalar var Z * BinInt.Z) with
+          | Cast r (Shiftl n x) =>
+            match invert_lower x return option (@scalar var Z * BinInt.Z) with
+            | Some x' =>
+              if (lower r =? 0) && (upper r =? wordmax-1) && (n =? half_bits)
+              then Some (x', half_bits)
+              else None
+            | None => None
+            end
+          | _ =>
+            match invert_upper s return _ with
+            | Some x => Some (x, -half_bits)
+            | None => None
+            end
+          end.
+
       Definition of_straightline_ident {s d} (idc : ident.ident s d)
         : forall t, range_type d -> @scalar var s -> (var d -> @expr var ident t) -> @expr var ident t :=
         match idc in ident.ident s d return forall t, range_type d -> scalar s -> (var d -> @expr var ident t) -> @expr var ident t with
         | ident.Z.add_get_carry_concrete w =>
           fun t r x f =>
             if w =? wordmax
-            then LetInAppIdentZZ r add x f
+            then
+              match x with
+              | Pair Z Z xl xr =>
+                match invert_shift xl, invert_shift xr with
+                | _, Some (xr', imm) => LetInAppIdentZZ r (add imm) (Pair xl xr') f
+                | Some (xl', imm), None => LetInAppIdentZZ r (add imm) (Pair xr xl') f
+
+                | None, None => LetInAppIdentZZ r (add 0) (Pair xl xr) f
+                end
+              | _ => dummy _
+              end
             else dummy _
         | ident.Z.add_with_get_carry_concrete w =>
           fun t r x f =>
             if w =? wordmax
-            then LetInAppIdentZZ r addc x f
+            then
+              match x with
+              | Pair (type.prod Z Z) Z (Pair Z Z xc xl) xr =>
+                match invert_shift xl, invert_shift xr with
+                | _, Some (xr', imm) => LetInAppIdentZZ r (addc imm) (Pair (Pair xc xl) xr') f
+                | Some (xl', imm), None => LetInAppIdentZZ r (addc imm) (Pair (Pair xc xr) xl') f
+
+                | None, None => LetInAppIdentZZ r (addc 0) (Pair (Pair xc xl) xr) f
+                end
+              | _ => dummy _
+              end
             else dummy _
         | ident.Z.sub_get_borrow_concrete w =>
           fun t r x f =>
             if w =? wordmax
-            then LetInAppIdentZZ r sub x f
+            then
+              match x with
+              | Pair Z Z xl xr =>
+                match invert_shift xr with
+                | Some (xr', imm) => LetInAppIdentZZ r (sub imm) (Pair xl xr') f
+                | None => LetInAppIdentZZ r (sub 0) (Pair xl xr) f
+                end
+              | _ => dummy _
+              end
             else dummy _
-        (* | ident.Z.land n => fun _ r => LetInAppIdentZ r (land n) *)
-        | ident.Z.shiftr n => fun _ r => LetInAppIdentZ r (shiftr n)
-        | ident.Z.shiftl n => fun _ r => LetInAppIdentZ r (shiftl n)
         | ident.Z.rshi_concrete w n =>
           fun _ r x f =>
             if w =? wordmax
@@ -8726,19 +8766,17 @@ Module PreFancy.
     Section interp.
       Local Notation low x := (Z.land x (wordmax_half_bits - 1)).
       Local Notation high x := (x >> half_bits).
+      Local Notation shift x imm := ((x << imm) mod wordmax).
 
       Definition interp_ident {s d} (idc : ident s d) : type.interp s -> type.interp d :=
         match idc with
-        | add => fun x => Z.add_get_carry_full wordmax (fst x) (snd x)
-        | addc => fun x => Z.add_with_get_carry_full wordmax (fst (fst x)) (snd (fst x)) (snd x)
+        | add imm => fun x => Z.add_get_carry_full wordmax (fst x) (shift (snd x) imm)
+        | addc imm => fun x => Z.add_with_get_carry_full wordmax (fst (fst x)) (snd (fst x)) (shift (snd x) imm)
+        | sub imm => fun x => Z.sub_get_borrow_full wordmax (fst x) (shift (snd x) imm)
         | mulll => fun x => low (fst x) * low (snd x)
         | mullh => fun x => low (fst x) * high (snd x)
         | mulhl => fun x => high (fst x) * low (snd x)
         | mulhh => fun x => high (fst x) * high (snd x)
-        | sub => fun x => Z.sub_get_borrow_full wordmax (fst x) (snd x)
-       (* | land n => fun x => Z.land x n *) (* only allowed inside select/mul? *)
-        | shiftr n => fun x => Z.shiftr x n
-        | shiftl n => fun x => Z.shiftl x n
         | rshi n => fun x => Z.rshi wordmax (fst x) (snd x) n
         | selc => fun x => Z.zselect (fst (fst x)) (snd (fst x)) (snd x)
         | selm => fun x => Z.zselect (Z.cc_m wordmax (fst (fst x))) (snd (fst x)) (snd x)
@@ -8855,50 +8893,33 @@ Module PreFancy.
 
       Inductive ok_ident : forall s d, scalar s -> range_type d -> ident.ident s d -> Prop :=
       | ok_add :
-          forall x : scalar (type.prod type.Z type.Z),
-            in_word_range (fst (get_range x)) ->
-            in_word_range (snd (get_range x)) ->
+          forall x y : scalar type.Z,
+            in_word_range (get_range x) ->
+            in_word_range (get_range y) ->
             ok_ident _
                      (type.prod type.Z type.Z)
-                     x
+                     (Pair x y)
                      (word_range, flag_range)
                      (ident.Z.add_get_carry_concrete wordmax)
       | ok_addc :
-          forall x : scalar (type.prod (type.prod type.Z type.Z) type.Z),
-            in_flag_range (fst (fst (get_range x))) ->
-            in_word_range (snd (fst (get_range x))) ->
-            in_word_range (snd (get_range x)) ->
+          forall c x y : scalar type.Z,
+            in_flag_range (get_range c) ->
+            in_word_range (get_range x) ->
+            in_word_range (get_range y) ->
             ok_ident _
                      (type.prod type.Z type.Z)
-                     x
+                     (Pair (Pair c x) y)
                      (word_range, flag_range)
                      (ident.Z.add_with_get_carry_concrete wordmax)
       | ok_sub :
-          forall x : scalar (type.prod type.Z type.Z),
-            in_word_range (fst (get_range x)) ->
-            in_word_range (snd (get_range x)) ->
+          forall x y : scalar type.Z,
+            in_word_range (get_range x) ->
+            in_word_range (get_range y) ->
             ok_ident _
                      (type.prod type.Z type.Z)
-                     x
+                     (Pair x y)
                      (word_range, flag_range)
                      (ident.Z.sub_get_borrow_concrete wordmax)
-     (* | ok_land :
-          forall (x : scalar type.Z) n,
-            in_word_range (get_range x) ->
-            0 <= n < wordmax ->
-            ok_ident type.Z type.Z x (ZRange.map (fun y => Z.land y n) (get_range x)) (ident.Z.land n)*)
-      | ok_shiftr :
-          forall (x : scalar type.Z) n r,
-            in_word_range (get_range x) ->
-            0 <= n <= log2wordmax ->
-            r = ZRange.map (fun y => Z.shiftr y n) (get_range x) ->
-            ok_ident type.Z type.Z x r (ident.Z.shiftr n)
-      | ok_shiftl :
-          forall (x : scalar type.Z) n,
-            in_word_range (get_range x) ->
-            0 <= n ->
-            upper (get_range x) * 2 ^ n <= wordmax - 1 ->
-            ok_ident type.Z type.Z x word_range (ident.Z.shiftl n)
       | ok_rshi :
           forall (x : scalar (type.prod type.Z type.Z)) n,
             in_word_range (fst (get_range x)) ->
@@ -9150,6 +9171,16 @@ Module PreFancy.
           | true => invert H; extract_ok_scalar' 1 x
           | _ => fail
           end
+        | H : ok_scalar (Pair (Pair x _) _) |- _ =>
+          match (eval compute in (2 <=? level)) with
+          | true => invert H; extract_ok_scalar' 1 x
+          | _ => fail
+          end
+        | H : ok_scalar (Pair (Pair _ x) _) |- _ =>
+          match (eval compute in (2 <=? level)) with
+          | true => invert H; extract_ok_scalar' 1 x
+          | _ => fail
+          end
         | H : ok_scalar (?g x) |- _ => invert H
         | H : ok_scalar (Pair x _) |- _ => invert H
         | H : ok_scalar (Pair _ x) |- _ => invert H
@@ -9304,9 +9335,6 @@ Module PreFancy.
           match goal with |- context[?x mod ?m] => pose proof (Z.mod_pos_bound x m ltac:(omega)) end.
           rewrite Z.div_sub_small by omega.
           split; break_match; lia. }
-        { apply has_range_shiftr; cbn [has_range]; omega. }
-        { eapply has_word_range_shiftl; eauto  with has_range omega.
-          apply in_word_range_spec ; omega. }
         { apply has_word_range_rshi; omega. }
         { rewrite Z.zselect_correct. break_match; omega. }
         { cbn [interp_scalar fst snd get_range] in *.
@@ -9423,6 +9451,73 @@ Module PreFancy.
           cbn; rewrite Pxi, Pyi; rewrite interp_cast_noop by auto; reflexivity.
       Qed.
 
+      Lemma has_word_range_mod_small x:
+        @has_range type.Z word_range x ->
+        x mod wordmax = x.
+      Proof.
+        cbv [has_range upper lower].
+        intros. apply Z.mod_small; omega.
+      Qed.
+
+      Lemma invert_shift_correct (s : scalar type.Z) x imm :
+        ok_scalar s ->
+        invert_shift consts s = Some (x, imm) ->
+        interp_scalar s = (interp_scalar x << imm) mod wordmax.
+      Proof.
+        (*
+        intros Hok ?; invert Hok;
+          try match goal with H : ok_scalar ?x, H' : context[Cast _ ?x] |- _ =>
+                          invert H end;
+          try match goal with H : ok_scalar ?x, H' : context[Shiftl _ ?x] |- _ =>
+                          invert H end;
+          try match goal with H : ok_scalar ?x, H' : context[Shiftl _ (Cast _ ?x)] |- _ =>
+                          invert H end;
+          try (cbn [invert_shift invert_upper invert_upper'] in *; discriminate).
+        {
+          repeat match goal with
+                 | _ => progress (cbn [invert_shift invert_upper invert_upper'
+                                                    interp_scalar fst snd] in * )
+                 | _ => rewrite interp_cast_noop by eauto using has_range_loosen
+                 | H : ok_scalar (Shiftr _ _) |- _ => apply has_range_interp_scalar in H
+                 | H : context [if ?x then _ else _] |- _ =>
+                   let Heq := fresh in case_eq x; intro Heq; rewrite Heq in H
+                 | H : _ |- _ => rewrite andb_true_iff in H; destruct H; Z.ltb_to_lt
+                 | H : Some _ = Some _ |- _ => progress (invert H)
+                 | _ => progress subst
+                 | _ => reflexivity
+                 | _ => discriminate
+                 end.
+          rewrite has_word_range_mod_small.
+          2:eauto using has_range_loosen.
+        }
+        {
+          repeat match goal with
+                 | _ => progress (cbn [invert_shift invert_upper invert_upper'
+                                                    invert_lower invert_lower'
+                                                    interp_scalar fst snd] in * )
+                 | _ => rewrite interp_cast_noop by eauto using has_range_loosen
+                 | H : ok_scalar (Shiftr _ _) |- _ => apply has_range_interp_scalar in H
+                 | H : ok_scalar (Shiftl _ _) |- _ => apply has_range_interp_scalar in H
+                 | H : ok_scalar (Land _ _) |- _ => apply has_range_interp_scalar in H
+                 | H : context [if ?x then _ else _] |- _ =>
+                   let Heq := fresh in case_eq x; intro Heq; rewrite Heq in H
+                 | H : _ |- _ => rewrite andb_true_iff in H; destruct H; Z.ltb_to_lt
+                 | H : Some _ = Some _ |- _ => progress (invert H)
+                 | _ => progress subst
+                 | _ => reflexivity
+                 | _ => discriminate
+                 end.
+      Qed.
+         *)
+        Admitted.
+
+      Local Ltac solve_commutative_replace :=
+        match goal with
+               | |- @eq (_ * _) ?x ?y =>
+                 replace x with (fst x, snd x) by (destruct x; reflexivity);
+                 replace y with (fst y, snd y) by (destruct y; reflexivity)
+        end; autorewrite with to_div_mod; solve [repeat (f_equal; try ring)].
+
       Lemma of_straightline_ident_correct s d t x r (idc : ident.ident s d) g :
         ok_ident s d x r idc ->
         ok_scalar x ->
@@ -9433,16 +9528,29 @@ Module PreFancy.
         pose proof wordmax_half_bits_pos.
         pose proof (ident_interp_has_range _ _ x r idc ltac:(assumption) ltac:(assumption)).
         induction H; try solve [auto using of_straightline_ident_mul_correct];
-          cbn [of_straightline_ident ident.interp ident.gen_interp invert_selm invert_sell] in *; intros;
-          rewrite ?Z.eqb_refl; cbn [interp interp_ident andb]; try destruct_scalar;
+          cbn [of_straightline_ident ident.interp ident.gen_interp
+                                     invert_selm invert_sell] in *;
+            intros; rewrite ?Z.eqb_refl; cbn [andb];
+            try match goal with |- context [invert_shift] => break_match end;
+            cbn [interp interp_ident]; try destruct_scalar;
             repeat match goal with
                    | _ => progress (cbn [fst snd interp_scalar] in * )
                    | _ => progress break_match; [ ]
+                   | _ => progress autorewrite with zsimplify_fast
                    | _ => rewrite interp_cast_noop with (r:=flag_range) in *
                        by (apply has_flag_range_cc_m'; auto; extract_ok_scalar)
                    | _ => rewrite interp_cast_noop with (r:=flag_range) in *
                        by (apply has_flag_range_land'; auto; extract_ok_scalar)
                    | H : _ = (_,_) |- _ => progress (inversion H; subst)
+                   | H : invert_shift _ _ = Some _ |- _ =>
+                     apply invert_shift_correct in H; [|extract_ok_scalar];
+                       rewrite <-H
+                   | H : has_range ?r  (?f ?x ?y) |- context [?f ?y ?x] =>
+                     replace (f y x) with (f x y) by solve_commutative_replace
+                   | _ => rewrite has_word_range_mod_small
+                       by (eapply has_range_loosen;
+                           [apply has_range_interp_scalar; extract_ok_scalar|];
+                           assumption)
                    | _ => rewrite interp_cast_noop by assumption
                    | _ => rewrite interp_cast2_noop by assumption
                    | _ => reflexivity
@@ -9513,25 +9621,32 @@ Module PreFancy.
     Notation "f @( y , x1 , x2 , x3 ); g "
       := (LetInAppIdentZZ (uint256, bool)%core f (Pair (Pair x1 x2) x3) (fun y => g))
            (at level 10, g at level 200, format "f @( y ,  x1 ,  x2 ,  x3 ); '//' g ").
-    Notation "f @( y , x1 , x2 , x3 ); g "
+    Notation "f @( y , x1 , x2 , x3 ); '#128' g "
       := (LetInAppIdentZZ (uint128, bool)%core f (Pair (Pair x1 x2) x3) (fun y => g))
-           (at level 10, g at level 200, format "f @( y ,  x1 ,  x2 ,  x3 ); '//' g ").
+           (at level 10, g at level 200, format "f @( y ,  x1 ,  x2 ,  x3 );  '#128' '//' g ").
     Notation "f @( y , x1 , x2 ); g "
       := (LetInAppIdentZ uint256 f (Pair x1 x2) (fun y => g))
            (at level 10, g at level 200, format "f @( y ,  x1 ,  x2 ); '//' g ").
     Notation "f @( y , x1 , x2 , x3 ); g "
       := (LetInAppIdentZ uint256 f (Pair (Pair x1 x2) x3) (fun y => g))
            (at level 10, g at level 200, format "f @( y ,  x1 ,  x2 ,  x3 ); '//' g ").
-    Notation "shiftL@( y , x , n ); g"
-      := (LetInAppIdentZ uint256 (shiftl n) (Lower{x}) (fun y => g))
-           (at level 10, g at level 200, format "shiftL@( y ,  x ,  n ); '//' g").
-    Notation "shiftR@( y , x , n ); g "
-      := (LetInAppIdentZ uint128 (shiftr n) x (fun y => g))
-           (at level 10, g at level 200, format "shiftR@( y ,  x ,  n ); '//' g ").
+    (* special cases for when the ident constructor takes a constant argument *)
+    Notation "add@( y , x1 , x2 , n ); g"
+      := (LetInAppIdentZZ (uint256, bool) (add n) (Pair x1 x2) (fun y => g))
+           (at level 10, g at level 200, format "add@( y ,  x1 ,  x2 ,  n ); '//' g").
+    Notation "addc@( y , x1 , x2 , x3 , n ); g"
+      := (LetInAppIdentZZ (uint256, bool) (addc n) (Pair (Pair x1 x2) x3) (fun y => g))
+           (at level 10, g at level 200, format "addc@( y ,  x1 ,  x2 ,  x3 ,  n ); '//' g").
+    Notation "addc@( y , x1 , x2 , x3 , n ); '#128' g"
+      := (LetInAppIdentZZ (uint128, bool) (addc n) (Pair (Pair x1 x2) x3) (fun y => g))
+           (at level 10, g at level 200, format "addc@( y ,  x1 ,  x2 ,  x3 ,  n );  '#128' '//' g").
+    Notation "sub@( y , x1 , x2 , n ); g"
+      := (LetInAppIdentZZ (uint256, bool) (sub n) (Pair x1 x2) (fun y => g))
+           (at level 10, g at level 200, format "sub@( y ,  x1 ,  x2 ,  n ); '//' g").
     Notation "rshi@( y , x1 , x2 , n ); g"
       := (LetInAppIdentZ _ (rshi n) (Pair x1 x2) (fun y => g))
            (at level 10, g at level 200, format "rshi@( y ,  x1 ,  x2 , n ); '//' g ").
-    Notation "'Ret' $ x" := (Scalar (Var tZ x)) (at level 10, format "'Ret'  $ x").
+    Notation "'ret' $ x" := (Scalar (Var tZ x)) (at level 10, format "'ret'  $ x").
     Notation "( x , y )" := (Pair x y) (at level 10, left associativity).
   End Notations.
 End PreFancy.
@@ -10159,30 +10274,24 @@ barrett_red256 =  fun var : type -> Type => λ x : var (type.type_primitive type
     mulhl@(y3, RegMuLow, $y1);
     mullh@(y4, RegMuLow, $y1);
     mulll@(y5, RegMuLow, $y1);
-    add@(y6, Straightline.expr.Cast uint256 (Straightline.expr.Shiftl 128 (Lower{$y3})), $y5);
-    addc@(y7, carry{$y6}, $y2, Straightline.expr.Cast uint128
-                                (Straightline.expr.Shiftr 128 ($y4)));
-    add@(y8, Straightline.expr.Cast uint256 (Straightline.expr.Shiftl 128 (Lower{$y4})), $y6);
-    addc@(y9, carry{$y8}, Straightline.expr.Cast uint128
-                            (Straightline.expr.Shiftr 128 ($y3)), $y7);
-    add@(y10, $y1, $y9);
-    addc@(y11, carry{$y10}, RegZero, $y0);
-    add@(y12, $y, $y10);
-    addc@(y13, carry{$y12}, RegZero, $y11);
+    add@(y6, $y5, $y3, 128);
+    addc@(y7, carry{$y6}, $y2, $y4, -128);
+    add@(y8, $y6, $y4, 128);
+    addc@(y9, carry{$y8}, $y7, $y3, -128);
+    add@(y10, $y1, $y9, 0);
+    addc@(y11, carry{$y10}, RegZero, $y0, 0); #128
+    add@(y12, $y, $y10, 0);
+    addc@(y13, carry{$y12}, RegZero, $y11, 0); #128
     rshi@(y14, $y13, $y12,1);
     mulhh@(y15, RegMod, $y14);
     mullh@(y16, RegMod, $y14);
     mulhl@(y17, RegMod, $y14);
     mulll@(y18, RegMod, $y14);
-    add@(y19, Straightline.expr.Cast uint256
-                (Straightline.expr.Shiftl 128 (Lower{$y16})), $y18);
-    addc@(y20, carry{$y19}, $y15, Straightline.expr.Cast uint128
-                                    (Straightline.expr.Shiftr 128 ($y17)));
-    add@(y21, Straightline.expr.Cast uint256
-                (Straightline.expr.Shiftl 128 (Lower{$y17})), $y19);
-    addc@(_, carry{$y21}, Straightline.expr.Cast uint128
-                            (Straightline.expr.Shiftr 128 ($y16)), $y20);
-    Straightline.expr.Scalar (Straightline.expr.Primitive (-1))
+    add@(y19, $y18, $y16, 128);
+    addc@(y20, carry{$y19}, $y15, $y17, -128);
+    add@(y21, $y19, $y17, 128);
+    addc@(_, carry{$y21}, $y20, $y16, -128);
+    Straightline.expr.Scalar (Straightline.expr.Primitive (-1))            
   *)
 End Barrett256.
 
@@ -10880,22 +10989,22 @@ montred256 = fun var : type -> Type => (λ x : var (type.type_primitive type.Z *
   (*
    mulhl@(y0, RegPInv, $x₁);
    mulll@(y1, RegPInv, $x₁);
-   add@(y2, Straightline.expr.Cast uint256 (Straightline.expr.Shiftl 128 (Lower{$y})), $y1);
-   add@(y3, Straightline.expr.Cast uint256 (Straightline.expr.Shiftl 128 (Lower{$y0})), $y2);
+   add@(y2, $y1, $y, 128);
+   add@(y3, $y2, $y0, 128);
    mulhh@(y4, RegMod, $y3);
    mullh@(y5, RegMod, $y3);
    mulhl@(y6, RegMod, $y3);
    mulll@(y7, RegMod, $y3);
-   add@(y8, Straightline.expr.Cast uint256 (Straightline.expr.Shiftl 128 (Lower{$y5})), $y7);
-   addc@(y9, carry{$y8}, $y4, Straightline.expr.Cast uint128 (Straightline.expr.Shiftr 128 ($y6)));
-   add@(y10, Straightline.expr.Cast uint256 (Straightline.expr.Shiftl 128 (Lower{$y6})), $y8);
-   addc@(y11, carry{$y10}, Straightline.expr.Cast uint128 (Straightline.expr.Shiftr 128 ($y5)), $y9);
-   add@(y12, $y10, $x₁);
-   addc@(y13, carry{$y12}, $y11, $x₂);
+   add@(y8, $y7, $y5, 128);
+   addc@(y9, carry{$y8}, $y4, $y6, -128);
+   add@(y10, $y8, $y6, 128);
+   addc@(y11, carry{$y10}, $y9, $y5, -128);
+   add@(y12, $y10, $x₁, 0);
+   addc@(y13, carry{$y12}, $y11, $x₂, 0);
    selc@(y14, carry{$y13}, RegZero, RegMod);
-   sub@(y15, $y13, $y14);
+   sub@(y15, $y13, $y14, 0);
    addm@(y16, $y15, RegZero, RegMod);
-   Ret $y16                  
+   ret $y16         
   *)
 End Montgomery256.
 
